stdlib/stdlib/src/lib.rs
@@ -21,4 +21,5 @@
 #![rr::export_include("result")]
 #![rr::export_include("rr_internal")]
 #![rr::export_include("vec")]
+#![rr::export_include("arithops")]
 
