theories/rust_typing/tests.v
@@ -1292,6 +1292,22 @@ Section test.
   Abort.
 End test.
 
+(** solve_llctx_remove_dead_aliases *)
+Section test.
+  Lemma llctx_remove_dead_aliases_test_1 κ :
+    ∃ L2, llctx_remove_dead_aliases [] L2 κ ∧ L2 = [].
+  Proof.
+    eexists; split; first solve_llctx_remove_dead_aliases; last done; solve [fail].
+  Abort.
+
+  Lemma llctx_remove_dead_aliases_test_2 κ1 κ2 κ3  :
+    ∃ L2, llctx_remove_dead_aliases [κ1 ⊑ₗ{0} []; κ2 ≡ₗ [κ3]] L2 κ3 ∧ L2 = [κ1 ⊑ₗ{0} []].
+  Proof.
+    eexists; split; first solve_llctx_remove_dead_aliases; last done; solve [fail].
+  Abort.
+
+End test.
+
 (** solve_bor_kind_outlives *)
 Section test.
   Context `{!typeGS Σ}.
